WIP on multi-arity methods.

lib/ADTInduction.v
@@ -5,19 +5,6 @@ Require Import Coq.Lists.List.
 
 Import ListNotations.
 
-(** Support for inducting over ADTs *)
-
-Fixpoint fromConstructor
-         {rep : Type}
-         {dom : list Type}
-         (const : constructorType rep dom)
-         (r : rep) : Prop :=
-  match dom return constructorType rep dom -> rep -> Prop with
-  | [ ] => fun const r => computes_to const r
-  | D :: dom' => fun const r =>
-                   exists (d : D), fromConstructor (const d) r
-  end const r.
-
 Fixpoint fromMethod' {rep : Type} {dom : list Type} :
   forall {cod : option Type}, methodType' rep dom cod -> rep -> Prop :=
   match dom return
@@ -33,23 +20,25 @@ Fixpoint fromMethod' {rep : Type} {dom : list Type} :
     fun cod meth r => exists d, fromMethod' (meth d) r
   end.
 
-Definition fromMethod
+Fixpoint fromMethod
+           {arity : nat}
            {rep : Type}
            {dom : list Type}
            {cod : option Type}
-           (meth : methodType rep dom cod)
-           (r : rep) : rep -> Prop :=
-  fromMethod' (meth r).
+           (meth : methodType arity rep dom cod)
+  : rep -> Prop :=
+  match arity return
+        methodType arity rep dom cod
+        -> rep -> Prop with
+  | 0 => fun meth' => fromMethod' meth'
+  | S n' => fun meth' r => exists r', fromMethod (meth' r') r
+  end meth.
 
 Inductive fromADT {sig} (adt : ADT sig) : Rep adt -> Prop :=
-  | fromADTConstructor :
-      forall (cidx : ConstructorIndex sig) (r : Rep adt),
-        fromConstructor (Constructors adt cidx) r
-        -> fromADT adt r
   | fromADTMethod :
       forall (midx : MethodIndex sig) (r r' : Rep adt),
         fromADT adt r
-        -> fromMethod (Methods adt midx) r r'
+        -> fromMethod (Methods adt midx) r'
         -> fromADT adt r'.
 
 Require Import Fiat.Common.IterateBoundedIndex.
@@ -64,17 +53,15 @@ Tactic Notation "ADT" "induction" ident(r) :=
     let H := fresh "H" in
     let H0 := fresh "H0" in
     let IHfromADT := fresh "IHfromADT" in
-    let offset :=
-        match goal with
-        | [ |- forall r : Rep _, fromADT _ r -> _ ] => 1
-        | [ |- forall r : Rep _, _ -> fromADT _ r -> _ ] => 2
-        | [ |- forall r : Rep _, _ -> _ -> fromADT _ r -> _ ] => 3
-        | [ |- forall r : Rep _, _ -> _ -> _ -> fromADT _ r -> _ ] => 4
-        end in
-    induction offset as [cidx r H|midx r r' H IHfromADT H0];
+    let induction_tac := (fun offset => induction offset as [cidx r H|midx r r' H IHfromADT H0]) in
+    match goal with
+    | [ |- forall r : Rep _, fromADT _ r -> _ ] => induction_tac 1
+    | [ |- forall r : Rep _, _ -> fromADT _ r -> _ ] => induction_tac 2
+    | [ |- forall r : Rep _, _ -> _ -> fromADT _ r -> _ ] => induction_tac 3
+    | [ |- forall r : Rep _, _ -> _ -> _ -> fromADT _ r -> _ ] => induction_tac 4
+    end;
     [ revert r H | revert r r' H H0 IHfromADT ];
     match goal with
-    | [ cidx : ConstructorIndex _ |- _ ] => pattern cidx
     | [ midx : MethodIndex _      |- _ ] => pattern midx
     end;
     apply Iterate_Ensemble_equiv';
@@ -92,7 +79,19 @@ Tactic Notation "ADT" "induction" ident(r) :=
     subst;
     eauto;
     match goal with
-    | [ cidx : ConstructorIndex _ |- _ ] => clear cidx
     | [ midx : MethodIndex _      |- _ ] => clear midx
     end
   end.
+
+Lemma ADT_ind {sig} (adt : ADT sig) :
+  forall (P : Ensemble (Rep adt))
+         (PM : forall midx r', fromMethod (Methods adt midx) r' -> P r'),
+         forall r : Rep adt, fromADT adt r -> P r.
+Proof.
+  intros.
+  induction H.
+  eapply PM.
+  exact H0.
+Qed.
+
+Definition ARep {sig} (adt : ADT sig) := { r : Rep adt | fromADT adt r }.
